\documentclass{article}
\usepackage[utf8]{inputenc}
\usepackage{setspace}
\usepackage{tikz}
\usetikzlibrary{positioning}
\usepackage{amsfonts}
\usepackage{amssymb}
\usepackage{amsmath}
\usepackage{amsthm}
\usepackage{systeme}
\usepackage{mathtools}
\usepackage{hyperref}

\begin{document}
\section*{Question 1}

~

\subsection*{Problem a}

~

\begin{equation*}
    \begin{split}
        &\text{Cayley's Theorem}:\\
        &\forall \text{ finite group }G,\exists H\subseteq S_n: |G|=n:G\cong H\\
        &H\subseteq S_n\implies H\subseteq S_{n+1}\\
        &\text{By induction}:\\
        &H\in S_\mathbb{Z} \\
        \Rightarrow&\forall \text{ finite group }G,\exists H\subseteq S_\mathbb{Z} : |G|=n:G\cong H\\
    \end{split}
\end{equation*}

~

\subsection*{Problem b}

~

\begin{equation*}
    \begin{split}
        &G\coloneqq \{\sigma^n|n\in\mathbb{Z}\}\\
        &\sigma:\mathbb{Z} \rightarrow\mathbb{Z} ,\sigma(x)\coloneqq x+1\\
        &G\text{ is a subgroup}:\\
        &Id=\sigma^0\in G \\
        &\forall \sigma^n(x)=x+n\in G,\exists \sigma^{-n}(x)=x-n:\sigma^n\circ \sigma^{-n}(x)=Id(x)=n\in G\\
        &\forall \sigma^m(x),\sigma^n(x)\in G,\exists \sigma^{m+n}(x)=x+m+n=\sigma^m\circ\sigma^n(x)\in G\\
        &\phi:\mathbb{Z} \rightarrow G\\
        &\phi(i)\coloneqq \sigma^i\\
    \end{split}
\end{equation*}

\begin{equation*}
    \begin{split}
        &\text{Injective}:\\
        &\exists i,j\in\mathbb{Z} :\phi(i)=\phi(j)\\
        &\sigma^i(x)=\sigma^j(x)\\
        &x+i=x+j\\
        \Rightarrow&i=j\\
        &\\
        &\text{Surjective}:\\
        &\forall \sigma^m\in G,\exists n=m\in\mathbb{Z} :\sigma^n=\sigma^m\in G\\
        &\\
        &\text{Homomorphism}:\\
        &\phi(m+n)=\sigma^{m+n}\\
        &\sigma^{m+n}=\sigma^m\cdot\sigma^n=\phi(m)\phi(n)\\
        &\phi(m+n)=\phi(m)\phi(n)\\
    \end{split}
\end{equation*}

~

\subsection*{Problem c}

~

\begin{equation*}
    \begin{split}
        &\text{Identity}:\\
        &Id\coloneqq \sigma(x)=x\forall x\in \mathbb{Z} \\
        \Rightarrow&Id\in H\\
        &\\
        &\text{Inverse}:\\
        &\exists \sigma\in H\\
        &\sigma^{-1}\circ\sigma(x)=x\\
        &\sigma\text{ moves only finitely many elements}\\
        \Rightarrow&\sigma^{-1}\text{ moves finitely many elements}\\
        \Rightarrow&\sigma^{-1}\in H,\forall \sigma\in H\\
        &\\
        &\text{Closure}:\\
        &\exists \sigma,\tau\in H\\
        &\text{Suppose }\sigma\text{ moves }m\text{ entries and }\tau\text{ moves }n\text{ entries}\\
        &\sigma\circ \tau\text{ moves at most }m+n\text{ entries}\\
        &m,n\text{ are finite}\implies m+n\text{ is finite}\\
        \Rightarrow&\forall \sigma,\tau \in H,\sigma\circ\tau \in H\\
        &\\
        \Rightarrow&H\text{ is a subgroup}\\
    \end{split}
\end{equation*}

~

\subsection*{Problem d}

~

\begin{equation*}
    \begin{split}
        &\sigma(x)=2-x\\
        &\sigma^2(x)=2-(2-x)=x\\
        \Rightarrow&\text{orbit is }\{\{1\},\{0,2\},...\{n,2-n\},...\}\\
        &\tau(x)=x+3\\
        &\tau^2(x)=x+2\times3\\
        \Rightarrow&\tau^n(x)=x+3n\\
        \Rightarrow&\text{orbit is }\{\{...,-3,0,3,...\},\{...,-2,1,4,...\},\{...,-1,2,5,...\}\}\\
    \end{split}
\end{equation*}

\newpage

\section*{Question 2}

~

\begin{equation*}
    \begin{split}
        &\sigma=\mu_1\mu_2...\mu_k\\
        &m\coloneqq ord(\sigma)\\
        \Rightarrow&\sigma^m=e\\
        &{\mu_1}^m{\mu_2}^m...{\mu_k}^m=e\\
        \Rightarrow&{\mu_1}^m={\mu_2}^m=...={\mu_k}^m=e\\
        &{\mu_1}^{l_1}={\mu_2}^{l_2}=...={\mu_k}^{l_k}=e\\
        \Rightarrow&l_1|m\land l_2|m\land...\land l_k|m\\
        \Rightarrow&m=n\times\text{lcm}(l_1,l_2,...,l_k)\\
        &\text{Since bigger common multiple is a multiple of least common multiple which cannot be the order}\\
        &m\text{ needs to be the smallest common multiple}\\
        \Rightarrow&ord(\sigma)=\text{lcm}(l_1,l_2,...,l_k)\\
    \end{split}
\end{equation*}

~

\newpage

\section*{Question 3}

~

\subsection*{Problem a}

~

\begin{equation*}
    \begin{split}
        &\text{Injective}:\\
        &\exists m,n\in G:c_x(m)=c_x(n)\\
        &xmx^{-1}=xnx^{-1}\\
        &x^{-1}xmx^{-1}=x^{-1}xnx^{-1}\\
        &mx^{-1}=nx^{-1}\\
        &mx^{-1}x=nx^{-1}x\\
        \Rightarrow&m=n\\
        \Rightarrow&\forall m,n\in G:c_x(m)=c_x(n)\implies m=n\\
        &\\
        &\text{Surjective}:\\
        &\forall g\in G,c_x(h)=xhx^{-1}=g\\
        &h=x^{-1}gx\in G\\
        \Rightarrow&\forall g\in G,\exists h\in G:c_x(h)=g\\
        \Rightarrow&c_x\text{ is bijective}\\
        \Rightarrow&c_x\text{ is a permutation}\\
        \Rightarrow&c_x\in S_G\\
    \end{split}
\end{equation*}

~

\subsection*{Problem b}

~

\begin{equation*}
    \begin{split}
        &\exists x,y\in G\\
        &c_{xy}(g)=xyg(xy)^{-1}=xygy^{-1}x^{-1}\\
        &c_x\circ c_y(g)=c_x(c_y(g))=xc_y(g)x^{-1}=xygy^{-1}x^{-1}\\
        \Rightarrow&c_{xy}=c_x\circ c_y\\
        &\phi\text{ is homomorphic}\\
        &\\
        &G\coloneqq \mathbb{Z} _3\\
        &1\ne2\\
        &\phi(1)=\phi(2)=Id\\
        &\phi\text{ is not injective}\\
    \end{split}
\end{equation*}

\newpage

\section*{Question 4}

~

\subsection*{Problem a}

~

\begin{equation*}
    \begin{split}
        &\text{Identity}:\\
        &\exists a\in G,e_G=a*a^{-1}\\
        &\phi\text{ is an homomorphism}\\
        \Rightarrow&\phi(a*_Ga^{-1})=\phi(a)*_H\phi(a^{-1})\\
        &\phi(a)*_H\phi(a^{-1})=\phi(a)*_H\phi(a)^{-1}=e_H\\
        \Rightarrow&\phi(e_G)=e_H\\
        \Rightarrow&e_G\in\ker\phi\\
        &\text{Inverse}:\\
        &\exists a\in\ker\phi\\
        \Rightarrow&\phi(a)=e_H\\
        &\phi(a*_Ga^{-1})=\phi(a)*_H\phi(a^{-1})=\phi(e_G)=e_H\\
        \Rightarrow&e_H*_H\phi(a^{-1})=e_H\\
        \Rightarrow&\phi(a^{-1})=e_H\\
        \Rightarrow&\forall a\in\ker\phi,a^{-1}\in \ker\phi\\
        &\text{Closure}:\\
        &\exists a,b\in\ker\phi\\
        &\phi(a)=\phi(b)=e_H\\
        &\phi(ab)=\phi(a)*_H\phi(b)=e_H*_He_H=e_H\\
        \Rightarrow&ab \in\ker\phi\\
        \Rightarrow&\forall a,b\in\ker\phi,ab\in\ker\phi\\
        \Rightarrow&\ker\phi\text{ is a subgroup of }G\\
    \end{split}
\end{equation*}

~

\subsection*{Problem b}

~

\begin{equation*}
    \begin{split}
        &g\in\ker\phi\\
        \Rightarrow&\phi(g)=e_H\\
        &\phi(c_x(g))=\phi(xgx^{-1})\\
        &\phi(xgx^{-1})=\phi(x)*_H\phi(g)*_H\phi(x^{-1})\leftarrow\text{homomorphism}\\
        \Rightarrow&\phi(c_x(g))=\phi(x)*_He*_H*_H\phi(x^{-1})=\phi(x)*_H\phi(x^{-1})\\
        &phi(x^{-1})=\phi(x)^{-1}\leftarrow\text{homomorphism}\\
        \Rightarrow&\phi(c_x(g))=\phi(x)*_H\phi(x)^{-1}=e_H\\
        \Rightarrow&c_x(g)=\in\ker\phi,\forall x\in G\\
    \end{split}
\end{equation*}

~

\subsection*{Problem c}

~

\begin{equation*}
    \begin{split}
        &\phi\text{ is injective}\implies \ker\phi=\{e_G\}:\\
        &\phi(e_G)=\phi(a*_Ga^{-1})=\phi(a)*_H\phi(a^{-1})=\phi(a)*_H\phi(a)^{-1}=e_H\\
        &\phi\text{ is injective}\\
        \Rightarrow&\forall a,b\in G, \phi(a)=\phi(b)\Rightarrow a=b\\
        &\text{Suppose}:\exists a\ne e_G\in G,\phi(a)=e_H\\
        &\phi(a)=\phi(e_G)\\
        &\forall a,b\in G, \phi(a)=\phi(b)\Leftrightarrow a=b\\
        \Rightarrow& a=e_G\nLeftrightarrow a\ne e_G\\
        \Rightarrow&\forall a\ne e_G\in G,\phi(a)\ne e_H\\
        \Rightarrow&\ker\phi=\{e_G\}\\
    \end{split}
\end{equation*}

\begin{equation*}
    \begin{split}
        &\ker\phi=\{e_G\}\implies\phi\text{ is injective} :\\
        &\text{Suppose}: \phi\text{ is not injective}\\
        \Rightarrow&\exists a\ne b\in G:\phi(a)=\phi(b)\\
        \Rightarrow&\phi(a)*_H\phi(a)^{-1}=\phi(b)*_H\phi(a)^{-1}\\
        \Rightarrow&e_H=\phi(b)*_H\phi(a)^{-1}\\
        &\phi(b)*_H\phi(a)^{-1}=\phi(b*a^{-1})\\
        &\phi(b*a^{-1})=e_H\\
        &\ker\phi=\{e_G\}\\
        \Rightarrow&b*a^{-1}=e_G\\
        \Rightarrow&b=a\nLeftrightarrow a\ne b\\
        \Rightarrow&\phi\text{ is injective}\\
        \Rightarrow&\phi\text{ is injective}\Leftrightarrow\ker\phi=\{e_G\}\\
    \end{split}
\end{equation*}

\newpage

\section*{Question 5}

~

\subsection*{Problem a}

~

\begin{equation*}
    \begin{split}
        &\text{Identity}:\\
        &Id:G\rightarrow G\\
        &Id(x) \coloneqq x\\
        &\text{Injection}:\\
        &\exists a,b\in G:f(a)=f(b)=m\\
        &f(a)=m\implies a=m\\
        &f(b)=m\implies b=m\\
        \Rightarrow&a=b\\
        \Rightarrow&\forall a,b\in G,f(a)=f(b)\implies a=b\\
        &\text{Surjection}:\\
        &\forall g\in G: Id(g)=g,g\in G\\
        \Rightarrow&Id\text{ is surjective}\\
        &\text{Homomorphism}:\\
        &\exists a,b\in G\\
        &Id(ab)=ab\\
        &Id(a)=a,Id(b)=b\\
        \Rightarrow&Id(ab)=Id(a)Id(b)\\
        \Rightarrow&Id\in \text{Aut}(G)\\
        &\\
        &\text{Inverse}:\\
        &\exists f\in\text{Aut}(G)\\
        &f\text{ is a bijection}\\
        \Rightarrow&f^{-1}\text{ is a bijection}\\
        &f(f^{-1}(mn))=mn\\
        &f(f^{-1}(m)f^{-1}(n))=f(f^{-1}(m))f(f^{-1}(n))=mn\\
        \Rightarrow&f(f^{-1}(mn))=f(f^{-1}(m)f^{-1}(n))\\
        \Rightarrow&f^{-1}(mn)=f^{-1}(m)f^{-1}(n)\leftarrow f\text{ is isomorphic}\\
        \Rightarrow&f^{-1}\text{ is isomorphic}\\
        \Rightarrow&f^{-1}\in \text{Aut}(G)\\
        &\forall f\in \text{Aut}(G),f^{-1}\in\text{Aut}(G)\\
    \end{split}
\end{equation*}

\begin{equation*}
    \begin{split}
        &\text{Closure}:\\
        &\exists f,G\in\text{Aut}(G)\\
        &f:G\rightarrow G,g:G\rightarrow G\\
        \Rightarrow&f\circ g:G\rightarrow G\\
        &f,g\text{ are bijections}\\
        \Rightarrow&f\circ g\text{ is bijective}\\
        &\exists a,b\in G\\
        &f\circ g(ab)=f(g(ab))\\
        &g(ab)=g(a)g(b)\\
        \Rightarrow&f(g(ab))=f(g(a))f(g(b))=f\circ g(a)f\circ g(b)\\
        \Rightarrow&f\circ g(ab)=f\circ g(a)f\circ g(b)\\
        \Rightarrow&\forall f,g\in \text{Aut}(G):f\circ g\in\text{Aut}(G)\\
        \Rightarrow&\text{Aut}(G)\subset S_G\\
    \end{split}
\end{equation*}

~

\subsection*{Problem b}

~

\begin{equation*}
    \begin{split}
        &x\in G\\
        \Rightarrow&x^{-1}\in G\\
        \Rightarrow&xgx^{-1}\in G,\forall g\in G\\
        \Rightarrow&c_x:G\rightarrow G\\
        &\text{Injection}:\\
        &\text{Suppose}:c_x(a)=c_x(b),a,b\in G\\
        \Rightarrow&xax^{-1}=xbx^{-1}\\
        \Rightarrow&x^{-1}xax^{-1}=x^{-1}xbx^{-1}\\
        &ax^{-1}=bx^{-1}\\
        &ax^{-1}x=bx^{-1}x\\
        \Rightarrow&a=b\\
        \Rightarrow&c_x(a)=c_x(b)\implies a=b\\
        &\text{Surjective}:\\
        &\forall g\in G, c_x(g)=xgx^{-1}\\
        &xgx^{-1}\in G\\
        \Rightarrow&\forall g\in G,\exists xgx^{-1}\in G:c_x(g)=xgx^{-1}\\
        &\text{Homomorphism}:\\
        &\exists a,b\in G\\
        &c_x(ab)=xabx^{-1}\\
        &c_x(a)=xax^{-1}\\
        &c_x(b)=xbx^{-1}\\
        &c_x(a)c_x(b)=xax^{-1}xbx^{-1}=xabx^{-1}\\
        \Rightarrow&c_x(ab)=c_x(a)c_x(b)\\
        \Rightarrow&c_x\in \text{Aut}(G)
    \end{split}
\end{equation*}

~

\subsection*{Problem c}

~

\begin{equation*}
    \begin{split}
        &G=\langle a\rangle\\
        \Rightarrow&\forall g\in G,\exists n\in \mathbb{Z} :g=a^n\\
        &\forall i\ne j\in[0,|\langle a\rangle|]\cap\mathbb{Z} :a^i\ne a^j\\
        &\phi\text{ is bijective}\\
        \Rightarrow&\phi(a^i)\ne\phi(a^j)\\
        \Rightarrow&\phi(a)^i\ne\phi(a)^j\\
        &\forall i\ne j\in[0,|\langle a\rangle|]\cap\mathbb{Z} :\phi(a)^i\ne\phi(a)^j\\
        \Rightarrow&\forall g\in G,\exists p\in\mathbb{Z} :g=\phi(a)^p\\
        \Rightarrow&G=\langle \phi(a)\rangle\\
    \end{split}
\end{equation*}

~

\subsection*{Problem d}

~

\begin{equation*}
    \begin{split}
        &\mathbb{Z}_4=\langle1\rangle=\langle3\rangle\\
        \Rightarrow&a=1\lor a=3\\
        &\mathbb{Z}_4=\langle\phi(a)\rangle\\
        \Rightarrow&\phi(a)=1\lor \phi(a)=3\\
        &\phi\text{ is homomorphic}\implies \phi(0)=0\\
        \Rightarrow&\text{Aut}(\mathbb{Z} _4)=\{\phi|\phi(0)=0\land\phi(1)=m\land\phi(3)=n,m\ne n\in\{1,3\}\}\\
        &\mathbb{Z} _5=\langle1\rangle=\langle2\rangle=\langle3\rangle=\langle4\rangle\\
        \Rightarrow&\phi(a)=1\lor \phi(a)=2\lor\phi(a)=3\lor\phi(a)=4\\
        &\phi\text{ is homomorphic}\implies \phi(0)=0\\
        \Rightarrow&\text{Aut}(\mathbb{Z} _5)=\{\phi|\phi(0)=0\land\phi(1)=m\land\phi(2)=n\land\phi(3)=p\land\phi(4)=q,m\ne n\ne p\ne q\in\{1,2,3,4\}\}\\
    \end{split}
\end{equation*}

\newpage

\section*{Reference}

~

Jeffery Shu
\end{document}